theories/LogicalRelation/Definition/Tree.v
@@ -1,0 +1,152 @@
+(** * LogRel.LogicalRelation.Definition.Tree : Definition of the logical relation for tree *)
+From Stdlib Require Import CRelationClasses.
+From LogRel Require Import Utils Syntax.All GenericTyping Monad.
+From LogRel.LogicalRelation.Definition Require Import Prelude Ne Nat.
+
+Set Primitive Projections.
+Set Universe Polymorphism.
+Set Polymorphic Inductive Cumulativity.
+
+
+(** ** Reducibility of natural number type *)
+Module TreeRedTy.
+
+  Record TreeRedTy `{ta : tag} `{WfType ta} `{RedType ta}
+    {Γ : context} {A B : term}
+  : Set :=
+  {
+    redL : [Γ |- A :⤳*: tTree] ;
+    redR : [Γ |- B :⤳*: tTree]
+  }.
+
+  Arguments TreeRedTy {_ _ _}.
+
+  Section TreeRedTy.
+  Context `{ta : tag} `{WfType ta} `{RedType ta}.
+
+  Definition whredL {Γ A B} : TreeRedTy Γ A B -> [Γ |- A ↘].
+  Proof. intros []; econstructor; tea; constructor. Defined.
+
+  Definition whredR {Γ A B} : TreeRedTy Γ A B -> [Γ |- B ↘].
+  Proof. intros []; econstructor; tea; constructor. Defined.
+
+  End TreeRedTy.
+
+End TreeRedTy.
+
+Export TreeRedTy(TreeRedTy, Build_TreeRedTy).
+Notation "[ Γ ||-Tree A ≅ B ]" := (TreeRedTy Γ A B) (at level 0, Γ, A at level 50).
+
+
+#[program]
+Instance WhRedTyTreeRedTy `{GenericTypingProperties} {Γ} : WhRedTyRel Γ (TreeRedTy Γ) :=
+  {|
+    whredtyL := fun A B RAB => TreeRedTy.whredL RAB ;
+    whredtyR := fun A B RAB => TreeRedTy.whredR RAB ;
+  |}.
+Next Obligation. destruct h; gtyping. Qed.
+
+Module TreeRedTmEq.
+Section TreeRedTmEq.
+  Context `{ta : tag} `{WfContext ta} `{WfType ta} `{ConvType ta}
+    `{RedType ta} `{Typing ta} `{ConvNeuConv ta} `{ConvTerm ta}
+    `{RedTerm ta} {Γ : context}.
+
+  Variant treeTmEqVariant : Set := RedEq | PropEq.
+
+  Inductive TreeTmEq : treeTmEqVariant -> term -> term -> Set :=
+  | Build_TreeRedTmEq {t u}
+    (nfL nfR : term)
+    (redL : [Γ |- t :⤳*: nfL : tTree])
+    (redR : [Γ |- u :⤳*: nfR : tTree ])
+    (eq : [Γ |- nfL ≅ nfR : tTree])
+    (prop : TreeTmEq PropEq nfL nfR) : TreeTmEq RedEq t u
+  | leafReq {n n'}
+    (Rn : NatRedTmEq Γ n n') :
+    TreeTmEq PropEq (tLeaf n) (tLeaf n')
+  | nodeReq {n n' tl tl' tr tr'}
+    (Rn : NatRedTmEq Γ n n')
+    (Rtl : TreeTmEq RedEq tl tl')
+    (Rtr : TreeTmEq RedEq tr tr') :
+    TreeTmEq PropEq (tNode n tl tr) (tNode n' tl' tr')
+  | neReq {ne ne'} : [Γ ||-NeNf ne ≅ ne' : tTree] -> TreeTmEq PropEq ne ne'.
+
+  Definition TreePropEq := (TreeTmEq PropEq).
+  Definition TreeRedTmEq := (TreeTmEq RedEq).
+
+  Definition TreeRedTmEq_destruct : forall (P : forall t u, TreeRedTmEq t u -> Type),
+    (forall t u nfL nfR redL redR eq prop, P t u (Build_TreeRedTmEq nfL nfR redL redR eq prop)) ->
+    forall t u (Rtu : TreeRedTmEq t u), P t u Rtu := fun P hBuild t u Rtu =>
+      match Rtu as Rtu' in TreeTmEq v t' u'
+        return (match v with
+          | RedEq => fun (R : TreeTmEq RedEq t' u') => P t' u' R
+          | _ => fun _ => unit end Rtu') with
+      | @Build_TreeRedTmEq t u nfL nfR redL redR eq prop => hBuild t u nfL nfR redL redR eq prop
+      | _ => tt end.
+
+  Definition TreePropEq_destruct : forall (P : forall t u, TreePropEq t u -> Type),
+    (forall n n' Rn, P (tLeaf n) (tLeaf n') (@leafReq n n' Rn)) ->
+    (forall n n' tl tl' tr tr' Rn Rtl Rtr, P (tNode n tl tr) (tNode n' tl' tr') (@nodeReq n n' tl tl' tr tr' Rn Rtl Rtr)) ->
+    (forall ne ne' Rne, P ne ne' (@neReq ne ne' Rne)) ->
+    forall t u (Rtu : TreePropEq t u), P t u Rtu := fun P hl hn hne t u Rtu =>
+      match Rtu as Rtu' in TreeTmEq v t' u'
+        return (match v with
+          | PropEq => fun (R : TreeTmEq PropEq t' u') => P t' u' R
+          | _ => fun _ => (unit : Type) end Rtu') with
+      | leafReq Rn => hl _ _ Rn
+      | nodeReq Rn Rtl Rtr => hn _ _ _ _ _ _ Rn Rtl Rtr
+      | neReq Rne => hne _ _ Rne
+      | _ => tt end.
+
+  Section Def.
+    Context `{!GenericTypingProperties _ _ _ _ _ _ _ _ _}.
+
+    Lemma TreePropEq_isTree {t t' : term} :
+      TreePropEq t t' -> isTree t × isTree t'.
+    Proof.
+      intros Rt. induction Rt  as [ | |?? []] using TreePropEq_destruct; split; constructor.
+      all: eapply convneu_whne; eassumption + now symmetry.
+    Defined.
+
+    Definition whnfL {t u} : TreePropEq t u -> whnf t.
+    Proof. intros []%TreePropEq_isTree; now eapply isTree_whnf. Qed.
+
+    Definition whnfR {t u} : TreePropEq t u -> whnf u.
+    Proof. intros []%TreePropEq_isTree; now eapply isTree_whnf. Qed.
+
+    Definition whredL {t u} : TreeRedTmEq t u -> [Γ |- t ↘ tTree].
+    Proof.
+      intros Rt.
+      induction Rt as [] using TreeRedTmEq_destruct; econstructor; tea; now eapply whnfL.
+    Defined.
+
+    Definition whredR {t u} : TreeRedTmEq t u -> [Γ |- u ↘ tTree].
+    Proof.
+      intros Rt.
+      destruct Rt as [] using TreeRedTmEq_destruct; econstructor; tea; now eapply whnfR.
+    Defined.
+
+  End Def.
+
+
+
+End TreeRedTmEq.
+
+Arguments TreeRedTmEq {_ _ _ _ _}.
+Arguments TreeTmEq {_ _ _ _ _}.
+End TreeRedTmEq.
+
+Export TreeRedTmEq(TreeRedTmEq,Build_TreeRedTmEq, TreePropEq, TreePropEq_isTree).
+
+
+Notation "[ Γ ||-Tree t ≅ u :Tree]" := (@TreeRedTmEq _ _ _ _ _ Γ t u).  (* (at level 0, Γ, t, u, A, RA at level 50). *)
+
+#[program]
+Instance TreeRedTmEqWhRed `{GenericTypingProperties} {Γ} : WhRedTmRel Γ tTree (TreeRedTmEq Γ) :=
+  {| whredtmL := fun t u Rtu => TreeRedTmEq.whredL Rtu ;
+    whredtmR := fun t u Rtu => TreeRedTmEq.whredR Rtu |}.
+Next Obligation.
+  now induction t, u, h using TreeRedTmEq.TreeRedTmEq_destruct.
+Qed.
+
+
