theories/LogicalRelation/Introductions/Tree.v
@@ -1,0 +1,319 @@
+
+From LogRel Require Import Utils Syntax.All GenericTyping Monad LogicalRelation.
+From LogRel.LogicalRelation Require Import Properties.
+From LogRel.LogicalRelation.Introductions Require Import Universe SimpleArr Application Nat.
+
+Set Universe Polymorphism.
+Set Printing Primitive Projection Parameters.
+
+Section Tree.
+Context `{GenericTypingProperties}.
+
+Set Printing Primitive Projection Parameters.
+
+Lemma treeRedTy {Γ} : [|- Γ] -> [Γ ||-Tree tTree ≅ tTree].
+Proof.
+  constructor; eapply redtywf_refl; gen_typing.
+Qed.
+
+Definition StreeRed {Γ l} (wfΓ : [|- Γ]) : [Γ ||-S<l> tTree] :=
+  LRTree_ l (treeRedTy wfΓ).
+
+Definition treeRed {Γ l} (wfΓ : [|- Γ]) : [Γ ||-<l> tTree] :=
+  WAd_return (StreeRed wfΓ).
+
+
+Lemma treeURedTm {Δ} (wfΔ : [|-Δ]) : URedTm zero Δ tTree.
+Proof.
+  exists tTree; [| constructor].
+  eapply redtmwf_refl; gen_typing.
+Defined.
+
+Lemma treeTermRed {Δ} (wfΔ : [|-Δ]) : [Δ ||-<one> tTree : U | LRU_ (redUOneCtx wfΔ)].
+Proof.
+  unshelve econstructor; try now eapply treeURedTm.
+  1: cbn; gtyping.
+  eapply redTyRecBwd; now eapply StreeRed.
+Defined.
+
+Lemma SleafRed {Γ l A A' B B' n n'} {NN : [Γ ||-Nat A ≅ A' ]} {NT : [Γ ||-Tree B ≅ B']} : [Γ ||-<l> n ≅ n' : _ | LRNat_ l NN] ->
+  [Γ ||-S<l> tLeaf n ≅ tLeaf n' : _ | LRTree_ l NT].
+Proof.
+  assert [|-Γ] by (pose (LRTree_ l NT); escape; gtyping).
+  intros Rn. inversion Rn; subst. escape.
+  eapply (Build_TreeRedTmEq (tLeaf n) (tLeaf n')).
+  1,2: eapply redtmwf_refl; eapply ty_leaf; gen_typing.
+  + destruct redL, redR.
+    eapply convtm_leaf; eapply convtm_exp; tea;
+    [eapply wft_term|eapply convty_term]; gtyping.
+  + now constructor.
+Defined.
+
+Lemma leafRed {Γ l n n'} (wfΓ : [|-Γ]) :
+  [Γ ||-< l > n ≅ n' : _ | natRed (l:=l) wfΓ] ->
+  [Γ ||-< l > tLeaf n ≅ tLeaf n' : _ | treeRed (l:=l) wfΓ].
+Proof.
+  intros Rn.
+  eapply (dSplit_bind_return Rn).
+  intros ??? onatRed oRn oir. cbn.
+  unshelve now eapply SirrLR, SleafRed, SirrLR, Rn.
+  4: eapply natRedTy.
+  4: eapply treeRedTy.
+  all: tea.
+Defined.
+
+Lemma SnodeRed {Γ l A A' B B' n n' tl tl' tr tr'}
+  {NN : [Γ ||-Nat A ≅ A']} {NT : [Γ ||-Tree B ≅ B']} :
+  [Γ ||-S<l> n ≅ n' : _ |LRNat_ l NN] ->
+  [Γ ||-S<l> tl ≅ tl' : _ |LRTree_ l NT] ->
+  [Γ ||-S<l> tr ≅ tr' : _ |LRTree_ l NT] ->
+  [Γ ||-S<l> tNode n tl tr ≅ tNode n' tl' tr' : _ |LRTree_ l NT].
+Proof.
+  assert [|-Γ] by (pose (LRTree_ l NT); escape; gtyping).
+  intros Rn Rtl Rtr; inversion Rn; inversion Rtl; inversion Rtr; subst.
+  escape; econstructor.
+  1,2: eapply redtmwf_refl; eapply ty_node; gen_typing.
+  + destruct redL, redR, redL0, redR0, redL1, redR1.
+    eapply convtm_node; eapply convtm_exp; tea;
+    first [eapply wft_term| eapply convty_term]; gtyping.
+  + now constructor.
+Defined.
+
+Lemma nodeRed {Γ l n n' tl tl' tr tr'} (wfΓ : [|-Γ]) :
+  [Γ ||-< l > n ≅ n' : _ | natRed (l:=l) wfΓ] ->
+  [Γ ||-< l > tl ≅ tl' : _ | treeRed (l:=l) wfΓ] ->
+  [Γ ||-< l > tr ≅ tr' : _ | treeRed (l:=l) wfΓ] ->
+  [Γ ||-< l > tNode n tl tr ≅ tNode n' tl' tr' : _ | treeRed (l:=l) wfΓ].
+Proof.
+  intros Rn Rtl Rtr.
+  eapply (dSplit_bind Rn).
+  intros ??? onatRed oRn.
+  unshelve eapply Wpackrefold; tea.
+  eapply (Split_wk_bind Rtl wfΔ ρ).
+  intros ??? oRtl.
+  unshelve eapply Wpackrefold; tea.
+  eapply (dSplit_wk_bind_return Rtr wfΞ (ρΞ ∘w ρ)).
+  intros Ω wfΩ ρΩ otree oRtr oirr.
+  rewrite 4 wk_comp_ren_on.
+  unshelve eapply SirrLR, SnodeRed; refold.
+  5: now eapply natRedTy.
+  3: now eapply treeRedTy.
+  tea.
+  + unshelve eapply SirrLR, Rn; tea.
+    1,2: now eapply overtree_PSh, overtree_PSh.
+  + unshelve eapply SirrLR, Rtl; tea.
+    now eapply overtree_PSh.
+  + unshelve eapply SirrLR, Rtr; tea.
+Qed.
+
+Lemma elimLeafHypTy_subst {P} σ :
+  elimLeafHypTy P[up_term_term σ] = (elimLeafHypTy P)[σ].
+Proof.
+  unfold elimLeafHypTy.
+  cbn. f_equal.
+  erewrite liftSubstComm'.
+  now rewrite up_liftSubst_eq.
+Qed.
+
+Lemma shift_upRen_eq : forall {t : term} {ρ : nat -> nat}, t⟨↑⟩⟨upRen_term_term ρ⟩ = t⟨ρ⟩⟨↑⟩.
+Proof.
+  intros t ρ.
+  now bsimpl.
+Qed.
+
+
+Lemma liftSubst_can {t u} : t[u]⇑ = t⟨upRen_term_term ↑⟩[u..].
+Proof.
+  rewrite <- up_single_subst.
+  f_equal.
+  rewrite rinstInst'_term.
+  now bsimpl.
+Qed.
+
+Lemma up_shift_up_eq t σ : t⟨upRen_term_term ↑⟩[up_term_term (up_term_term σ)] = t[up_term_term σ]⟨upRen_term_term ↑⟩.
+Proof.
+  now bsimpl.
+Qed.
+
+Lemma up_shift_one_eq t a : t⟨upRen_term_term ↑⟩[up_term_term a..] = t.
+Proof.
+  now bsimpl.
+Qed.
+
+Lemma elimNodeHypTy_subst {P} σ :
+  elimNodeHypTy P[up_term_term σ] = (elimNodeHypTy P)[σ].
+Proof.
+  unfold elimNodeHypTy.
+  cbn. do 4 f_equal; [|f_equal]. 
+  + now rewrite shift_up_eq, up_shift_up_eq.
+  + now rewrite shift_up_eq, 2 up_shift_up_eq.
+  + now rewrite 2 liftSubst_can, 2 shift_upRen_eq,
+    2 shift_up_eq, singleSubstComm', 3 up_shift_up_eq.
+Qed.
+
+Lemma liftSubst_singleSubst_eq {t u v: term} : t[u]⇑[v..] = t[u[v..]..].
+Proof. now bsimpl. Qed.
+
+Section STreeElimRedEq.
+  Context {Γ l P Q hl hl' hn hn'}
+    (NT : [Γ ||-Tree tTree ≅ tTree])
+    (RT := LRTree_ _ NT)
+    (WtP : [Γ ,, tTree |- P])
+    (WtQ : [Γ ,, tTree |- Q])
+    (eqPQ : [Γ,, tTree |- P ≅ Q])
+    (RPQext : forall n n' (Rn : [Γ ||-S<l> n ≅ n' : _ | RT]),
+      [Γ ||-<l> P[n..] ≅ Q[n'..]])
+    (RPQl : [Γ ||-<l> elimLeafHypTy P ≅ elimLeafHypTy Q])
+    (Rhl : [Γ ||-<l> hl ≅ hl' : _ | RPQl])
+    (RPQn : [Γ ||-<l> elimNodeHypTy P ≅ elimNodeHypTy Q])
+    (Rhn : [Γ ||-<l> hn ≅ hn' : _ | RPQn ]) .
+
+  Let RPext : forall n n' (Rn : [Γ ||-S<l> n ≅ n' : _ | RT]),
+      [Γ ||-<l> P[n..] ≅ P[n'..]].
+  Proof.
+    intros; etransitivity; [|symmetry];  eapply RPQext; tea; now eapply urefl.
+  Qed.
+
+(*   Lemma redΠcod Γ F F' G G'  *)
+
+  Lemma StreeElimRedEq :
+    (forall t t' (Rt : [Γ ||-S<l> t ≅ t' : _ | RT]),
+      [Γ ||-<l> tTreeElim P hl hn t ≅ tTreeElim Q hl' hn' t' : _ |  (RPQext _ _ Rt) ]).
+  Proof.
+    eassert ([|-Γ]) as wfΓ by (escape; gtyping).
+    intros t t' Rt.
+    set (RP := RPQext t t' Rt); clearbody RP.
+    induction Rt as [ ??????? prop ih| | ??????? Rtl ihl Rtr ihr| ].
+    - set (Rtu := Build_TreeRedTmEq _ _ redL redR eq prop : [Γ ||-S<l> t ≅ u : _ | RT]).
+      pose proof (redTmFwd' Rtu) as []; eapply redSubstTmEq.
+      + unshelve eapply irrLRConv, ih;
+        first [eapply RPQext | eapply RPext]; tea; now symmetry.
+      + escape; eapply redtm_treeelim; tea; gen_typing.
+      + escape; eapply redtm_treeelim; tea; [..| gtyping].
+        1,2: now eapply ty_conv.
+    - change [Γ ||-S<l> n ≅ n' : _ | LRNat_ l (natRedTy wfΓ)] in Rn.
+      intros; eapply redSubstTmEq; cycle 1.
+      + escape; eapply redtm_treeElimLeaf; tea.
+      + escape; eapply redtm_treeElimLeaf; tea.
+        1,2: now eapply ty_conv.
+      + eapply Wpack_return in Rn as WRn.
+        eapply irrLREq, appcongTerm, WRn.
+        2: eapply Rhl.
+        now bsimpl. Unshelve.
+        now rewrite 2 liftSubst_singleSubst_eq.
+    - change [Γ ||-S<l> n ≅ n' : _ | LRNat_ l (natRedTy wfΓ)] in Rn.
+      change [Γ ||-S<l> tl ≅ tl' : _ | RT] in Rtl.
+      change [Γ ||-S<l> tr ≅ tr' : _ | RT] in Rtr.
+      intros; eapply redSubstTmEq; cycle 1.
+      + escape; eapply redtm_treeElimNode; tea.
+      + escape; eapply redtm_treeElimNode; tea.
+        1,2: now eapply ty_conv.
+      + unshelve eapply simple_appcongTerm, ihr.
+        1: now eapply RPQext.
+        1: now eapply ArrRedTy; eapply RPQext; [..| eapply (SnodeRed (NN:=natRedTy wfΓ))].
+        unshelve eapply simple_appcongTerm, ihl.
+        1: now eapply RPQext.
+        1: now eapply ArrRedTy, ArrRedTy; eapply RPQext; [..| eapply (SnodeRed (NN:=natRedTy wfΓ))].
+        eapply Wpack_return in Rn as WRn.
+        eapply Wpack_return in Rtl as WRtl.
+        eapply Wpack_return in Rtr as WRtr.
+        epose proof (codSubst RPQn WRn) as RPQnn; cbn in RPQnn.
+        epose proof (codSubst RPQnn WRtl) as RPQnntl; cbn in RPQnntl.
+        epose proof (codSubst RPQnntl WRtr) as RPQnntltr; cbn in RPQnntltr.
+        eapply irrLREq, appcongTerm, WRtr; [shelve|..].
+        eapply irrLREq, appcongTerm, WRtl;  [shelve|..].
+        eapply irrLREq, appcongTerm, WRn;  [shelve|..].
+        eapply Rhn. Unshelve.
+        12: cbn; reflexivity.
+        9: cbn; reflexivity.
+        4:{ cbn; f_equal; [|f_equal].
+          * now rewrite 2 shift_up_eq, shift_one_eq, up_shift_one_eq.
+          * now rewrite 3 shift_up_eq, up_shift_up_eq, 2 up_shift_one_eq.
+          * rewrite 2 shift_upRen_eq, 6 shift_up_eq, liftSubst_can, 3 singleSubstComm'.
+            rewrite 3 up_shift_up_eq, 3 up_shift_one_eq.
+            do 4 f_equal. cbn.
+            now rewrite shift_up_eq, 3 shift_one_eq. }
+        6,7: eapply RPQnn.
+        3,4: eapply RPQnntl.
+        1: eapply RPQnntltr.
+    - epose proof (SneNfTermEq RT r).
+      escape.
+      eapply irrLR.
+      eapply neNfTermEq; constructor.
+      + now eapply ty_treeElim.
+      + eapply ty_conv.
+        eapply ty_treeElim; tea.
+        * now eapply ty_conv.
+        * now eapply ty_conv.
+        * now symmetry.
+      + destruct r; now eapply convneu_treeElim.
+      Unshelve.
+      2: now eapply lrefl.
+  Qed.
+
+End STreeElimRedEq.
+
+Section TreeElimRedEq.
+  Context {Γ l P Q}
+    (wfΓ : [|- Γ])
+    (WtP : [Γ ,, tTree |- P])
+    (WtQ : [Γ ,, tTree |- Q])
+    (eqPQ : [Γ,, tTree |- P ≅ Q])
+    (RPQext : forall Δ (wfΔ : [|-Δ]) (ρ : Δ ≤ Γ) t t' (Rt : [Δ ||-<l> t ≅ t' : _ | treeRed (l:=l) wfΔ ]),
+      [Δ ||-<l> P⟨wk_up tTree ρ⟩[t..] ≅ Q⟨wk_up tTree ρ⟩[t'..]]).
+
+
+  Let RPQextnow : forall t t',
+    [Γ ||-<l> t ≅ t' : _ | treeRed (Γ := Γ) (l:=l) wfΓ] -> [Γ ||-<l> P[t..] ≅ Q[t'..]].
+  Proof.
+    intros t t' Rtt'.
+    epose (RPQ := RPQext Γ wfΓ wk_id t t' Rtt').
+    replace P with P⟨wk_id (Γ:=Γ,,tTree)⟩ by eapply wk_id_ren_on.
+    now replace Q with Q⟨wk_id (Γ:=Γ,,tTree)⟩ by eapply wk_id_ren_on.
+  Qed.
+
+  Context {hl hl' hn hn'}
+    (RPQl : [Γ ||-<l> elimLeafHypTy P ≅ elimLeafHypTy Q])
+    (Rhl : [Γ ||-<l> hl ≅ hl' : _ | RPQl ])
+    (RPQn : [Γ ||-<l> elimNodeHypTy P ≅ elimNodeHypTy Q])
+    (Rhn : [Γ ||-<l> hn ≅ hn' : _ | RPQn ]).
+
+  Let RPext : forall Δ (wfΔ : [|-Δ]) (ρ : Δ ≤ Γ) t t' (Rn : [Δ ||-<l> t ≅ t' : _ | treeRed (l:=l) wfΔ]),
+      [Δ ||-<l> P⟨wk_up tTree ρ⟩[t..] ≅ P⟨wk_up tTree ρ⟩[t'..]].
+  Proof.
+    intros; etransitivity; [|symmetry];  eapply RPQext; tea; now eapply urefl.
+  Qed.
+
+
+  Lemma treeElimRedEq t t' (Rt : [Γ ||-<l> t ≅ t' : _ | treeRed wfΓ]):
+      [Γ ||-<l> tTreeElim P hl hn t ≅ tTreeElim Q hl' hn' t' : _ | RPQextnow _ _ Rt].
+  Proof.
+    eapply (dSplit_bind Rt).
+    intros Δ wfΔ ρ oRT oRt.
+    eapply Wpackrefold.
+    eassert [|-Δ,,tTree] as wfΔT by (eapply wfc_cons; gtyping).
+    rewrite <- 2wk_treeElim.
+    eapply irrLREq, StreeElimRedEq; refold.
+    1: symmetry; eapply subst_ren_wk_up.
+    Unshelve.
+    + now eapply wft_wk.
+    + now eapply wft_wk.
+    + now eapply convty_wk.
+    + unshelve eapply irrLREq, wkLRTm, Rhl; tea.
+      symmetry; eapply wk_elimLeafHypTy.
+    + unshelve eapply irrLREq, wkLRTm, Rhn; tea.
+      symmetry; eapply wk_elimNodeHypTy.
+    + easy.
+    + now eapply treeRedTy.
+    + clear dependent t; clear t'; intros t t' Rt.
+      eapply (RPQext _ wfΔ), Wpack_return, SirrLR, Rt.
+    + now unshelve now eapply SirrLREq, Rt.
+    + rewrite 2 wk_elimLeafHypTy.
+      now eapply wkLRTy.
+    + rewrite 2 wk_elimNodeHypTy.
+      now eapply wkLRTy.
+  Qed.
+
+End TreeElimRedEq.
+
+End Tree.
