theories/Validity/Introductions/Split.v
@@ -1,0 +1,438 @@
+From Stdlib Require Import ssrbool.
+From LogRel Require Import Utils Syntax.All GenericTyping LogicalRelation Monad.
+From LogRel.LogicalRelation Require Import Properties.
+From LogRel.LogicalRelation.Introductions Require Import Poly Pi Nat Bool.
+From LogRel.Validity Require Import Validity Irrelevance Properties Universe Poly ValidityTactics Nat Bool.
+
+Section FSnoc.
+  Context `{GenericTypingProperties}.
+
+  Lemma FequivValid {Γ Γ' : context} (VΓ : [||-v Γ ≅ Γ']) : Γ =ε Γ'.
+  Proof.
+    induction Γ, Γ', VΓ using validity_rect; tea.
+  Qed.
+
+(*   Lemma FSnocValidTy {Γ} {new} A . *)
+
+  Lemma validFSnoc {Γ Γ' : context} (VΓ : [||-v Γ ≅ Γ']) {new : newnat Γ} {new' : newnat Γ'} {b}:
+    new = new' :> nat -> [||-v Γ,, new ↦ b ≅ Γ',, new' ↦ b].
+  Proof.
+    intros.
+    induction Γ, Γ', VΓ using validity_rect.
+    + eapply validEmpty, Fequiv_Fup; now symmetry.
+    + change [||-v Γ,, new ↦ b,,A ≅ Γ',, new' ↦ b,,A'].
+      eapply validSnoc.
+      constructor.
+      intros * h.
+      eapply (wkValidTy (wk_Fstep (new : newnat Γ) b wk_id)) in VA.
+      rewrite 2!wk_Fstep_ren_on,  2!wk_id_ren_on in VA.
+      eapply VA, h.
+      Unshelve.
+      easy.
+  Defined.
+
+  Lemma irrSubstEq {Γ0 Γ0' Γ1 Γ1'} {VΓ0 : [||-v Γ0 ≅ Γ0']} {VΓ1 : [||-v Γ1 ≅ Γ1']} :
+    Γ0 = Γ1 ->
+    forall {Δ} (wfΔ : [|- Δ]) {σ σ'},
+    [Δ ||-v σ ≅ σ' : _ | VΓ0 | wfΔ ] ->
+    [Δ ||-v σ ≅ σ' : _ | VΓ1 | wfΔ ].
+  Proof.
+    intros <- *.
+    eapply convSubst.
+  Qed.
+
+  Lemma validFSnocSubst_in {Γ Γ' : context} (VΓ : [||-v Γ ≅ Γ']) {new : newnat Γ} {new' : newnat Γ'} {b σ σ'} {Δ wfΔ}
+    ( e: new = new' :> nat) :
+    [Δ ||-v σ ≅ σ' : _ | VΓ | wfΔ] -> in_Fctx Δ new b -> [Δ ||-v σ  ≅ σ' : Γ,, new ↦ b | validFSnoc VΓ e | wfΔ].
+  Proof.
+    revert σ σ'.
+    induction Γ, Γ', VΓ using validity_rect; intros σ σ' [] hin.
+    + constructor.
+      now eapply Fwk_new.
+    + econstructor.
+      now eapply irrLR.
+      Unshelve.
+      now unshelve now eapply irrelevanceSubst, IHVΓ.
+  Qed.
+
+  Lemma FSnocSubst {Γ Γ' : context} (VΓ : [||-v Γ ≅ Γ']) :
+  forall {σ σ' Δ new b} (wfΔ : [|- Δ]) (wfΔnew : [|- Δ,, new ↦ b]),
+  [Δ ||-v σ ≅ σ' : Γ | VΓ | wfΔ ] ->
+  [Δ,,new ↦ b ||-v σ ≅ σ' : Γ | VΓ | wfΔnew ].
+  Proof.
+    intros ???????. revert σ σ'.
+    induction Γ, Γ', VΓ using validity_rect; intros ?? [].
+    + constructor.
+      now eapply Fwk_Fstep.
+    + unshelve econstructor.
+      now eapply IHVΓ.
+      eapply (irrLREq (A:= A[↑ >> σ]⟨wk_Fstep new b wk_id⟩)).
+      etransitivity; [eapply wk_Fstep_ren_on | eapply wk_id_ren_on].
+      rewrite <- (wk_id_ren_on Δ (σ var_zero)), <- (wk_id_ren_on Δ (σ' var_zero)),
+        <- 2(wk_Fstep_ren_on new b).
+      eapply wkLR, eqHead.
+      Unshelve.
+      now eapply wfc_consF.
+  Qed.
+
+  Lemma validFSnocSubst_notin {Γ Γ' : context} (VΓ : [||-v Γ ≅ Γ']) {new : newnat Γ} {new' : newnat Γ'} {b σ σ'} {Δ wfΔ}
+    ( e: new = new' :> nat) (Vσσ' : [Δ ||-v σ ≅ σ' : _ | VΓ | wfΔ]) (notinΔ : not_in_Fctx Δ new) :
+      let newΔ := Build_newnat Δ new notinΔ in [Δ,,newΔ ↦ b ||-v σ  ≅ σ' : Γ,, new ↦ b | validFSnoc VΓ e | wfc_consF wfΔ].
+  Proof.
+    intros ?.
+    eapply validFSnocSubst_in.
+    now eapply FSnocSubst.
+    cbn.
+    eapply in_hereF.
+  Qed.
+
+(*   Lemma validTy_shf {Γ} {wfΓ : [|-Γ]} {VΓ : [||-v Γ]} {l A B} :
+    shf (fun Δ wfΔ ρ => forall (VΔ : [||-v Δ]), [Δ ||-v< l > A⟨ρ⟩ ≅ B⟨ρ⟩ | VΔ]).
+  Proof.
+    intros ???? ht hf ?.
+(*     set (new' := Build_newnat Δ' new (wk_new_notin new (lFwk (FequivValid VΔ)))). *)
+    specialize (ht (validFSnoc VΔ eq_refl)).
+    specialize (hf (validFSnoc VΔ eq_refl)).
+    rewrite 2 !wk_Fstep_ren_on in ht,hf.
+    constructor.
+    intros Ξ wfΞ ???.
+    destruct (decide_in Ξ new) as [ [] hin | hnotin].
+    - eapply ht.
+      eapply validFSnocSubst_in; tea.
+    - eapply hf.
+      eapply validFSnocSubst_in; tea.
+    - eapply WAd_split.
+      + eapply ht.
+        now unshelve eapply validFSnocSubst_notin, vσσ'.
+      + eapply hf.
+        now unshelve eapply validFSnocSubst_notin, vσσ'.
+  Qed.
+
+  Lemma Split_bind_validTy {Γ} {wfΓ : [|-Γ]} {VΓ : [||-v Γ]} {l A B C } (hC : Split (wfΓ:=wfΓ) C) :
+    (forall Δ (VΔ : [||-v Δ]) (ρ : Δ ≤ Γ), overtree hC Δ -> [Δ ||-v< l > A⟨ρ⟩ ≅ B⟨ρ⟩ | VΔ]) ->
+    [Γ ||-v< l > A ≅ B | VΓ].
+  Proof.
+    intros hAB.
+    rewrite <- (wk_id_ren_on Γ A), <- (wk_id_ren_on Γ B).
+    unshelve eapply (Split_bind_alg validTy_shf hC), wfΓ; tea.
+    intros ??? ohC ?.
+    now eapply hAB.
+  Qed. *)
+End FSnoc.
+
+Section Split.
+Context `{GenericTypingProperties}.
+
+Lemma validTySplit {Γ l A B} {new}
+  {VΓ : [||-v Γ]} {VΓt : [||-v Γ,,new ↦ true]} {VΓf : [||-v Γ,,new ↦ false]}:
+  [Γ,,new ↦ true ||-v<l> A ≅ B| VΓt] ->
+  [Γ,,new ↦ false  ||-v<l> A ≅ B| VΓf] ->
+  [Γ ||-v<l> A ≅ B| VΓ].
+Proof.
+  intros VAt VAf.
+  econstructor.
+  intros Δ wfΔ σ σ' Vσσ'.
+  destruct (decide_in Δ new) as [[] hin|hnotin].
+  + now unshelve now eapply VAt, convSubst, validFSnocSubst_in.
+  + now unshelve now eapply VAf, convSubst, validFSnocSubst_in.
+  + eapply WAd_split.
+    - now unshelve now eapply VAt, convSubst, validFSnocSubst_notin.
+    - now unshelve now eapply VAf, convSubst, validFSnocSubst_notin.
+Qed.
+
+
+Lemma Wpack_split {Γ l A B t u new}
+  {RAt : [Γ,, new ↦ true ||-< l > A ≅ B]} {RAf : [Γ,, new ↦ false ||-< l > A ≅ B]} :
+  [Γ,, new ↦ true ||-< l > t ≅ u  : A | RAt] -> [Γ,, new ↦ false ||-< l > t ≅ u  : A | RAf] ->
+  [Γ ||-< l > t ≅ u : A | WAd_split RAt RAf].
+Proof.
+  intros Rtt Rtf.
+  assert (wftrue : [|-Γ,, new ↦ true]) by apply RAt.
+  assert (wffalse : [|-Γ,, new ↦ false]) by apply RAf.
+  assert (wfΓ : [|-Γ]) by now eapply wfc_split.
+  epose proof (Split_shf Γ wfΓ wk_id new).
+  cbn in X.
+  eapply Split_hom_PSh.
+  2: eapply X; clear X.
+  + intros ??? ?.
+    rewrite wk_comp_runit in X0.
+    exact X0.
+  + eapply (dSplit_bind_return Rtt).
+    intros ??? oRAt oRtt osplit.
+    rewrite <- 2!wk_comp_ren_on, 2!wk_Fstep_ren_on, 2!wk_id_ren_on.
+    unshelve eapply SirrLREq, Rtt, oRtt; tea.
+    now rewrite <- wk_comp_ren_on, wk_Fstep_ren_on, wk_id_ren_on.
+  + eapply (dSplit_bind_return Rtf).
+    intros ??? oRAt oRtf osplit.
+    rewrite <- 2!wk_comp_ren_on, 2!wk_Fstep_ren_on, 2!wk_id_ren_on.
+    unshelve eapply SirrLREq, Rtf, oRtf; tea.
+    now rewrite <- wk_comp_ren_on, wk_Fstep_ren_on, wk_id_ren_on.
+Qed.
+
+Lemma validTmSplit {Γ l A t u} {new}
+  {VΓ : [||-v Γ]} {VΓt : [||-v Γ,,new ↦ true]} {VΓf : [||-v Γ,,new ↦ false]}
+  {VAt : [Γ,,new ↦ true ||-v<l> A | VΓt]} {VAf : [Γ,,new ↦ false ||-v<l> A| VΓf]}:
+  [Γ,,new ↦ true ||-v<l> t ≅ u : A | VΓt | VAt] ->
+  [Γ,,new ↦ false  ||-v<l> t ≅ u : A | VΓf | VAf] ->
+  [Γ ||-v<l> t ≅ u : A | VΓ | validTySplit VAt VAf].
+Proof.
+  intros Vtt Vtf.
+  econstructor.
+  intros ?????.
+  destruct (decide_in Δ new) as [[] hin|hnotin].
+  + unshelve eapply irrLR, Vtt; tea.
+    now unshelve now eapply convSubst, validFSnocSubst_in.
+  + unshelve eapply irrLR, Vtf; tea.
+    now unshelve now eapply convSubst, validFSnocSubst_in.
+  + eapply irrLR, Wpack_split.
+    - unshelve eapply Vtt.
+      1: now eapply wfc_consF.
+      now unshelve now eapply convSubst, validFSnocSubst_notin.
+    - unshelve eapply Vtf.
+      1: now eapply wfc_consF.
+      now unshelve now eapply convSubst, validFSnocSubst_notin.
+Qed.
+
+Lemma validCtxSplit {Γ new} :
+  [||-v Γ,,new ↦ true] -> [||-v Γ,,new ↦ false] -> [||-v Γ].
+Proof.
+  intros VΓt VΓf.
+  induction Γ using Tctx_induction.
+  + now eapply validEmpty.
+  + rewrite <- cons_Fcons in VΓt, VΓf.
+    destruct (invValidity VΓt) as (lt&At'&Γt'&VΓt'&VAt'&et&et').
+    revert VΓt' VAt' et'; pattern Γt', At', et.
+    eapply cons_eq_inversion; clear dependent At'; clear Γt'.
+    intros; cbn in et'; subst.
+    destruct (invValidity VΓf) as (lf&Af'&Γf'&VΓf'&VAf'&ef&ef').
+    revert VΓf' VAf' ef'; pattern Γf', Af', ef.
+    eapply cons_eq_inversion; clear dependent Af'; clear Γf'.
+    intros; cbn in ef'; subst.
+    now unshelve now eapply validSnoc, validTySplit; eapply embValidTyOne.
+Qed.
+
+  Section Strong.
+
+  Context {Γ wfΓ l}
+    (NN : [Γ ||-Nat tNat ≅ tNat])
+    (RN := LRNat_ l NN)
+    (RB := boolRed (Γ:=Γ) (l:=l) wfΓ).
+
+Lemma ty_nSucc {n t} :
+  [Γ |- t : tNat] ->
+  [Γ |- nSucc n t : tNat].
+Proof.
+  intros ht; induction n.
+  - tea.
+  - cbn. now eapply ty_succ.
+Qed.
+
+Lemma convtm_nSucc {n t t'} :
+  [Γ |- t ≅ t': tNat] ->
+  [Γ |- nSucc n t ≅ nSucc n t': tNat].
+Proof.
+  intros ht; induction n.
+  - tea.
+  - cbn. now eapply convtm_succ.
+Qed.
+
+Lemma nat_to_termReq n : NatPropEq Γ (nat_to_term n) (nat_to_term n).
+Proof.
+  induction n.
+  - constructor.
+  - cbn; constructor.
+    econstructor.
+    4: eapply IHn.
+    1,2: now constructor; [| eapply redtm_refl]; eapply ty_nSucc, ty_zero.
+    now eapply convtm_nSucc, convtm_zero.
+Qed.
+
+Lemma nSuccReq n {t t'} : [Γ||-Nat t ≅ t':Nat] -> [Γ ||-Nat nSucc n t ≅ nSucc n t' :Nat].
+Proof.
+  intros Rt.
+  induction n.
+  - eassumption.
+  - cbn. unshelve eapply SsuccRed, IHn.
+    4: eapply NN.
+    tea.
+Qed.
+
+Lemma nSuccswap n t : nSucc n (tSucc t) = tSucc (nSucc n t).
+Proof.
+  induction n.
+  + reflexivity.
+  + cbn. now rewrite IHn.
+Qed.
+
+Inductive NatPropEqInst : term -> term -> Set :=
+  | natReqInst n : NatPropEqInst (nat_to_term n) (nat_to_term n)
+  | neReqInst n neL neR : [Γ ||-NeNf neL ≅ neR : tNat] ->
+      NatPropEqInst (nSucc n neL) (nSucc n neR).
+
+Record NatRedTmEqInst tL tR : Set :=
+  {
+    nfLInst : term ;
+    nfRInst : term ;
+    redLInst : forall n, [Γ |- tAlpha (nSucc n tL) :⤳*: tAlpha (nSucc n nfLInst) : tBool] ;
+    redRInst : forall n, [Γ |- tAlpha (nSucc n tR) :⤳*: tAlpha (nSucc n nfRInst) : tBool ] ;
+(*     eqInst : [Γ |- nfL ≅ nfR : tBool] ; *)
+    propInst : NatPropEqInst nfLInst nfRInst
+  }.
+
+
+Lemma redtmwf_alphaSubst {t u n} :
+  [ Γ |- t :⤳*: u : tNat ] ->
+  [ Γ |- tAlpha (nSucc n t) :⤳*: tAlpha (nSucc n u) : tBool ].
+Proof.
+  intros ht.
+  econstructor.
+  + eapply ty_alpha, ty_nSucc, ht.
+  + eapply redtm_alphaSubst, ht.
+Qed.
+
+Definition natRed_toInst :
+  (forall tL tR (Rt : [Γ ||-Nat tL ≅ tR :Nat]), NatRedTmEqInst tL tR) ×
+  (forall tL tR (propt : NatPropEq Γ tL tR), NatRedTmEqInst tL tR).
+Proof.
+  apply NatRedEqInduction.
+  + intros tL tR ???? _ _ [dnfL dnfR redL' redR' prop].
+    econstructor.
+    3: eapply prop.
+    all: now etransitivity; [eapply redtmwf_alphaSubst |].
+  + econstructor.
+    3: eapply (natReqInst 0).
+    all: now intros n; eapply redtmwf_refl; eapply ty_alpha, ty_nSucc, ty_zero.
+  + intros tL tR Rt [dnfL dnfR redL redR prop].
+    eexists (tSucc dnfL) (tSucc dnfR).
+    - intros n. rewrite 2nSuccswap.
+      refine (redL (S n)).
+    - intros n. rewrite 2nSuccswap.
+      refine (redR (S n)).
+    - destruct prop.
+      * eapply (natReqInst (S n)).
+      * now eapply (neReqInst (S n)).
+  + intros neL neR Rne.
+    exists neL neR.
+    1,2: intros; eapply redtmwf_refl, ty_alpha, ty_nSucc, Rne.
+    now eapply (neReqInst 0).
+Defined.
+
+
+Lemma SAlphaRedEq (tL tR: term):
+  [Γ ||-S< l > tL ≅ tR: tNat | SnatRed (l:=l) wfΓ] -> [Γ ||-< l > tAlpha tL ≅ tAlpha tR: tBool|boolRed (l:=l) wfΓ].
+Proof.
+  intros.
+  eapply natRed_toInst in X.
+  destruct X as [dnfL dnfR redL redR prop].
+  induction prop.
+  + specialize (redL 0); specialize (redR 0); cbn in redL, redR.
+    destruct redL, redR.
+    eapply redSubstTmEq; tea.
+    destruct (decide_in Γ n) as [b hin | hnotin].
+    - eapply redSubstTmEq.
+      2,3: now eapply redtm_alpha.
+      destruct b.
+      eapply trueRed.
+      eapply falseRed.
+    - set (new := Build_newnat _ n hnotin).
+      eassert (wfΓt :[ |-[ ta ] Γ,, new ↦ true])
+         by now eapply wfc_consF.
+      eassert (wfΓf :[ |-[ ta ] Γ,, new ↦ false])
+         by now eapply wfc_consF.
+      eapply irrLR, (Wpack_split (new:=new)).
+      * eapply redSubstTmEq.
+        2,3: now eapply redtm_alpha, in_hereF.
+        now unshelve eapply trueRed.
+      * eapply redSubstTmEq.
+        2,3: now eapply redtm_alpha, in_hereF; eapply wfc_consF.
+        now unshelve eapply falseRed.
+      Unshelve. tea.
+  + specialize (redL 0); specialize (redR 0); cbn in redL, redR.
+    destruct redL, redR.
+    eapply redSubstTmEq; tea.
+    eapply neNfTermEq; econstructor; tea.
+    eapply convneu_alpha, r.
+Qed.
+
+End Strong.
+
+
+Lemma AlphaRedEq {Γ : context} {wfΓ : [|-Γ]} {l} (n n': term):
+  [Γ ||-< l > n ≅ n': tNat | natRed (l:=l) wfΓ] -> [Γ ||-< l > tAlpha n ≅ tAlpha n': tBool|boolRed (l:=l) wfΓ].
+Proof.
+  intros Rnn'.
+  eapply (dSplit_bind Rnn').
+  intros ??? onatRed oRnn'.
+  eapply Wpackrefold.
+  change (tAlpha ?n)⟨?ρ⟩ with (tAlpha n⟨ρ⟩).
+  eapply irrLR, SAlphaRedEq.
+  now unshelve now eapply SirrLR, Rnn'.
+  Unshelve. all:tea.
+Qed.
+
+Lemma validAlpha (Γ : context) (VΓ : [||-v Γ ≅ Γ])  (n n': term) l:
+  [Γ ||-v< l > n ≅ n': tNat | VΓ| natValid VΓ] -> [Γ ||-v< l > tAlpha n ≅ tAlpha n': tBool |VΓ|boolValid VΓ].
+Proof.
+  intros Vn.
+  econstructor.
+  intros.
+  instValid Vσσ'.
+  change (tAlpha ?n)[?σ] with (tAlpha n[σ]).
+  now eapply irrLR, AlphaRedEq.
+Qed.
+
+Lemma digammaRedEq (Γ : context) (n : nat) (b : bool) (wfΓ :[ |- Γ]) l:
+  in_Fctx Γ n b ->  [Γ ||-<l> tAlpha (nat_to_term n) ≅ bool_to_term b : tBool | boolRed (l:=l) wfΓ].
+Proof.
+  intros hin.
+  eapply redSubstLeftTmEq.
+  2: now eapply redtm_alpha, hin.
+  destruct b.
+  eapply trueRed.
+  eapply falseRed.
+Qed.
+
+Lemma nSucc_subst n t σ : (nSucc n t)[σ] = nSucc n (t[σ]).
+Proof.
+  induction n.
+  + reflexivity.
+  + cbn. now f_equal.
+Qed.
+
+Lemma nat_to_term_subst n σ : (nat_to_term n)[σ] = nat_to_term n.
+Proof. eapply nSucc_subst. Qed.
+
+Lemma bool_to_term_subst b σ : (bool_to_term b)[σ] = bool_to_term b.
+Proof. induction b; reflexivity. Qed.
+
+Inductive Box (P : SProp) : Type := box (p : P) : Box P.
+
+Lemma validSubst_ε  {Γ Γ' σ σ' Δ} (VΓ : [||-v Γ ≅ Γ' ]) (wfΔ : [|- Δ]) :
+  [Δ ||-v σ ≅ σ' : Γ | VΓ | wfΔ] -> Δ ≤ε Γ.
+Proof.
+  intros. enough (Box (Δ ≤ε Γ)) as [] by tea.
+  revert σ σ' X.
+  indValid VΓ.
+  + intros * [].
+    now constructor.
+  + intros *.
+    intros IH σ σ' [].
+    eapply IH, eqTail.
+Qed.
+
+Lemma validDigamma  (Γ : context) (VΓ : [||-v Γ ≅ Γ])  (n : nat) (b:bool) l:
+  in_Fctx Γ n b -> [Γ ||-v< l > tAlpha (nat_to_term n) ≅ bool_to_term b : tBool |VΓ|boolValid VΓ].
+Proof.
+  intros hin.
+  econstructor.
+  intros.
+  change (tAlpha ?n)[?σ] with (tAlpha n[σ]).
+  rewrite nat_to_term_subst, bool_to_term_subst.
+  eapply irrLR, digammaRedEq.
+  eapply validSubst_ε in Vσσ'.
+  now eapply Vσσ'.
+  Unshelve. all: tea.
+Qed.
+
+End Split.
+
