theories/Validity/Introductions/Tree.v
@@ -1,0 +1,267 @@
+From LogRel Require Import Utils Syntax.All GenericTyping LogicalRelation.
+From LogRel.LogicalRelation Require Import Properties.
+From LogRel.LogicalRelation.Introductions Require Import Universe SimpleArr Application Tree.
+From LogRel.Validity Require Import Validity Irrelevance Properties Universe Pi SimpleArr Var Application Nat.
+
+Set Universe Polymorphism.
+Set Printing Primitive Projection Parameters.
+
+Section Tree.
+Context `{GenericTypingProperties}.
+
+Set Printing Primitive Projection Parameters.
+
+Lemma treeValid {Γ Γ' l} (VΓ : [||-v Γ ≅ Γ']) : [Γ ||-v<l> tTree | VΓ].
+Proof.
+  unshelve econstructor; intros; now eapply treeRed.
+Defined.
+
+Lemma treeValidU {Γ} (VΓ : [||-v Γ]):  [Γ ||-v<one> tTree : U | VΓ | UValid VΓ].
+Proof.
+  constructor; intros; eapply Wpack_return, treeTermRed.
+Qed.
+
+Lemma leafValid {Γ Γ' l n n'} (VΓ : [||-v Γ ≅ Γ'])
+  (Vn : [Γ ||-v<l> n ≅ n' : tNat | VΓ | natValid VΓ]) :
+  [Γ ||-v<l> tLeaf n ≅ tLeaf n' : tTree | VΓ | treeValid VΓ].
+Proof.
+  constructor; intros; cbn -[Wpack]; instValid Vσσ'.
+  unshelve eapply leafRed; tea.
+Qed.
+
+Lemma leafValid' {Γ Γ' A A' l n n'} (VΓ : [||-v Γ ≅ Γ'])
+  (VT : [Γ ||-v<l> A ≅ A' | VΓ])
+  (eqA : A = tTree)
+  (Vn : [Γ ||-v<l> n ≅ n' : tNat | VΓ | natValid VΓ]) :
+  [Γ ||-v<l> tLeaf n ≅ tLeaf n' : A | VΓ | VT].
+Proof.
+  subst.
+  constructor; intros; cbn -[Wpack]; instValid Vσσ'; eapply irrLR.
+  unshelve eapply leafRed, irrLR; cycle 4; tea.
+  Unshelve. tea.
+Qed.
+
+(* Lemma nodeValid' {Γ Γ' A A' l n n'} (VΓ : [||-v Γ ≅ Γ'])
+  (VN : [Γ ||-v<l> A ≅ A' | VΓ])
+  (eqA : A = tNat)
+  (Veqn : [Γ ||-v<l> n ≅ n' : A | VΓ | VN]) :
+  [Γ ||-v<l> tSucc n ≅ tSucc n' : A | VΓ | VN].
+Proof.
+  subst.
+  constructor; intros; cbn -[Wpack]; instValid Vσσ'; eapply irrLR.
+  unshelve eapply succRed, irrLR; cycle 4; tea.
+  Unshelve. tea.
+Qed. *)
+
+Lemma nodeValid {Γ Γ' l n n' tl tl' tr tr'} (VΓ : [||-v Γ ≅ Γ'])
+  (Vn : [Γ ||-v<l> n ≅ n' : tNat | VΓ | natValid VΓ])
+  (Vtl : [Γ ||-v<l> tl ≅ tl' : tTree | VΓ | treeValid VΓ])
+  (Vtr : [Γ ||-v<l> tr ≅ tr' : tTree | VΓ | treeValid VΓ]) :
+  [Γ ||-v<l> tNode n tl tr ≅ tNode n' tl' tr' : tTree | VΓ | treeValid VΓ].
+Proof.
+  constructor; intros; cbn; instValid Vσσ'.
+  unshelve eapply nodeRed; tea.
+Qed.
+
+Lemma nodeValid' {Γ Γ' l A A' n n' tl tl' tr tr'} (VΓ : [||-v Γ ≅ Γ'])
+  (VT : [Γ ||-v<l> A ≅ A' | VΓ])
+  (eqA : A = tTree)
+  (Vn : [Γ ||-v<l> n ≅ n' : tNat | VΓ | natValid VΓ])
+  (Vtl : [Γ ||-v<l> tl ≅ tl' : tTree | VΓ | treeValid VΓ])
+  (Vtr : [Γ ||-v<l> tr ≅ tr' : tTree | VΓ | treeValid VΓ]) :
+  [Γ ||-v<l> tNode n tl tr ≅ tNode n' tl' tr' : A | VΓ | VT].
+Proof.
+  subst.
+  constructor; intros; cbn -[Wpack]; instValid Vσσ'; eapply irrLR.
+  unshelve eapply nodeRed; tea.
+Qed.
+
+
+Section TreeElimValid.
+  Context {Γ Γ' l}
+    (VΓ : [||-v Γ ≅ Γ'])
+    (VT := treeValid (l:=l) VΓ)
+    (VΓT := validSnoc VΓ VT).
+
+  Lemma elimLeafHypTyValid {P Q}
+    (VP : [Γ ,, tTree ||-v<l> P ≅ Q| VΓT]) :
+    [Γ ||-v<l> elimLeafHypTy P  ≅ elimLeafHypTy Q | VΓ].
+  Proof.
+    unfold elimLeafHypTy.
+    unshelve eapply PiValid.
+    1: eapply natValid.
+    eapply substLiftS; tea. cbn.
+    eapply leafValid'; [easy|].
+    change tNat with tNat⟨↑⟩.
+    eapply var0Valid'.
+  Qed.
+
+  Lemma elimNodeHypTyValid {P Q}
+    (VP : [Γ ,, tTree ||-v<l> P ≅ Q| VΓT]) :
+    [Γ ||-v<l> elimNodeHypTy P  ≅ elimNodeHypTy Q | VΓ].
+  Proof.
+    unfold elimNodeHypTy.
+    unshelve eapply PiValid.
+    1: eapply natValid.
+    unshelve eapply PiValid.
+    1: eapply treeValid.
+    unshelve eapply PiValid.
+    1: eapply treeValid.
+    eapply simpleArrValid.
+    erewrite <- 2wk1_ren_on.
+    eapply wkValidTy.
+    replace P⟨upRen_term_term ↑⟩ with P⟨wk_up (Δ:=Γ) tTree (wk1 tNat)⟩ by now bsimpl.
+    replace Q⟨upRen_term_term ↑⟩ with Q⟨wk_up (Δ:=Γ) tTree (wk1 tNat)⟩ by now bsimpl.
+    now eapply wkValidTy.
+    eassert (hupup : forall t, t⟨upRen_term_term ↑⟩⟨upRen_term_term ↑⟩ = t⟨wk_up (Δ:=Γ) tTree (wk1 tNat)⟩⟨wk_up (Δ:=Γ,,tNat) tTree (wk1 tTree)⟩) by (intros; now bsimpl).
+    eapply simpleArrValid.
+    rewrite 2 hupup.
+    now do 2 eapply wkValidTy.
+    eapply substLiftS.
+    rewrite 2 hupup.
+    now do 2 eapply wkValidTy.
+    eapply nodeValid'; [easy|..].
+    + eapply varnValid.
+      change tNat with tNat⟨↑⟩⟨↑⟩.
+      repeat constructor.
+    + eapply varnValid.
+      change tTree with tTree⟨↑⟩.
+      repeat constructor.
+    + eapply varnValid.
+      constructor.
+    Unshelve.
+    2,4,8: unshelve eapply validSnoc, treeValid.
+    3,6,9: unshelve eapply validSnoc, natValid.
+    14: unshelve eapply treeValid.
+    all: tea.
+  Qed.
+
+  Lemma treeElimCongValid {P P' hl hl' hn hn'}
+    (VP : [Γ ,, tTree ||-v<l> P ≅ P' | VΓT ])
+    (Vhl : [Γ ||-v<l> hl ≅ hl' : _ | VΓ | elimLeafHypTyValid VP ])
+    (Vhn : [Γ ||-v<l> hn ≅ hn' : _ | VΓ | elimNodeHypTyValid VP])
+    {t t'}
+    (Vt : [Γ ||-v<l> t ≅ t' : tTree | VΓ | VT])
+    (VPt := substS VP Vt)
+    : [Γ ||-v<l> tTreeElim P hl hn t ≅ tTreeElim P' hl' hn' t' : _ | VΓ | VPt].
+  Proof.
+    pose proof (elimLeafHypTyValid VP).
+    pose proof (elimNodeHypTyValid VP).
+    constructor; intros; instValid Vσσ'; epose proof (Vuσ := liftSubst' VT Vσσ').
+    instValid Vuσ; cbn -[elimLeafHypTy elimLeafHypTyValid elimNodeHypTy elimNodeHypTyValid Wpack] in *.
+    eapply irrLREq. 1: now rewrite singleSubstComm'.
+    unshelve eapply treeElimRedEq; tea.
+    4-6: now escape.
+    + clear dependent t; clear dependent t'; intros Ξ wfΞ ρΞ ???.
+      rewrite 2eq_upren', 2!up_single_subst; eapply validTyExt; tea.
+      unshelve eapply wkSubst in Vσσ' as VρΞ; tea.
+      now unshelve econstructor.
+    + now rewrite 2!elimLeafHypTy_subst.
+    + now rewrite 2!elimNodeHypTy_subst.
+    + eapply irrLREq; tea; now rewrite elimLeafHypTy_subst.
+    + eapply irrLREq; tea; now rewrite elimNodeHypTy_subst.
+  Qed.
+End TreeElimValid.
+
+Lemma treeElimValid {Γ Γ' l P hl hl' hn hn' t t'}
+    (VΓ : [||-v Γ ≅ Γ'])
+    (VT := treeValid (l:=l) VΓ)
+    (VΓT := validSnoc VΓ VT)
+    (VP : [Γ ,, tTree ||-v<l> P | VΓT])
+    (Vhl : [Γ ||-v<l> hl ≅ hl' : _ | VΓ | elimLeafHypTyValid VΓ VP])
+    (Vhn : [Γ ||-v<l> hn ≅ hn' : _ | VΓ | elimNodeHypTyValid VΓ VP])
+    (Vt : [Γ ||-v<l> t ≅ t' : _ | VΓ | VT])
+    (VPt := substS VP Vt):
+    [Γ ||-v<l> tTreeElim P hl hn t : _ | VΓ | VPt].
+Proof. now eapply lrefl, treeElimCongValid. Qed.
+
+Section TreeElimRedValid.
+  Context {Γ Γ' l}
+    (VΓ : [||-v Γ ≅ Γ'])
+    (VN := natValid (l:=l) VΓ)
+    (VT := treeValid (l:=l) VΓ)
+    (VΓT := validSnoc VΓ VT)
+    { P P' hl hl' hn hn'}
+    (VP : [Γ ,, tTree ||-v<l> P ≅ P' | VΓT ])
+    (Vhl : [Γ ||-v<l> hl ≅ hl' : _ | VΓ | elimLeafHypTyValid VΓ VP])
+    (Vhn : [Γ ||-v<l> hn ≅ hn' : _ | VΓ | elimNodeHypTyValid VΓ VP]).
+
+  Lemma treeElimLeafValid {n}
+    (Vn : [Γ ||-v<l> n : tNat | VΓ | VN])
+    (VPLn := substS VP (leafValid _ Vn)) :
+    [Γ ||-v<l> tTreeElim P hl hn (tLeaf n) ≅ tApp hl n : _ | VΓ | VPLn].
+  Proof.
+    eapply redSubstValid.
+    * constructor; intros; rewrite singleSubstComm'.
+      instValid Vσσ'; instValid (liftSubst' VT Vσσ'); escape.
+      eapply redtm_treeElimLeaf; tea; refold.
+      + now rewrite elimLeafHypTy_subst.
+      + now rewrite elimNodeHypTy_subst.
+    * eapply lrefl, appcongValid'.
+      1: eapply Vhl.
+      2: now bsimpl.
+      unshelve eapply irrValidTm, Vn; tea.
+      2: eapply irrValidTy; tea.
+      all: now eapply lrefl.
+  Qed.
+
+  Lemma substSΠ' { F F' G G' t u}
+    {VF : [Γ ||-v< l > F ≅ F' |VΓ]}
+    (VΠ : [Γ ||-v<l> tProd F G ≅ tProd F' G' | VΓ])
+    (Vt : [Γ ||-v<l> t ≅ u : F | VΓ |VF]) :
+    [_ ||-v<l> G[t..] ≅ G'[u..] | VΓ].
+  Proof.
+    unshelve eapply substSΠ, irrValidTm, Vt.
+    3: eapply VΠ.
+    3: eapply lrefl, irrValidTy, VF.
+    all: now eapply lrefl.
+  Qed.
+
+  Lemma treeElimNodeValid {n tl tr}
+    (Vn : [Γ ||-v<l> n : tNat | VΓ | VN])
+    (Vtl : [Γ ||-v<l> tl : tTree | VΓ | VT])
+    (Vtr : [Γ ||-v<l> tr : tTree | VΓ | VT])
+    (VPnode := substS VP (nodeValid _ Vn Vtl Vtr)) :
+    [Γ ||-v<l> tTreeElim P hl hn (tNode n tl tr) ≅
+      tApp (tApp (tApp (tApp (tApp hn n) tl) tr) (tTreeElim P hl hn tl)) (tTreeElim P hl hn tr) :
+       _ | VΓ | VPnode].
+  Proof.
+    eapply redSubstValid.
+    * constructor; intros; rewrite singleSubstComm'.
+      instValid Vσσ'; instValid (liftSubst' VT Vσσ'); escape.
+      eapply redtm_treeElimNode; tea; refold.
+      + now rewrite elimLeafHypTy_subst.
+      + now rewrite elimNodeHypTy_subst.
+    * epose proof (VPn := substSΠ' (elimNodeHypTyValid VΓ VP) Vn); cbn in VPn.
+      epose proof (VPtl := substSΠ' VPn Vtl); cbn in VPtl.
+      epose proof (VPtr := substSΠ' VPtl Vtr); cbn in VPtr.
+      eapply lrefl, simple_appValid.
+      2: now unshelve now eapply treeElimCongValid.
+      eapply simple_appValid.
+      2: now unshelve now eapply treeElimCongValid.
+      eapply appcongValid'; [|shelve..].
+      eapply appcongValid'; [|shelve..].
+      now eapply appcongValid'; [|shelve..].
+      Unshelve.
+      21: reflexivity.
+      16: reflexivity. all: refold.
+      8:{ cbn. f_equal; [|f_equal].
+          + now rewrite 2shift_up_eq, shift_one_eq, up_shift_one_eq.
+          + now rewrite 3shift_up_eq, up_shift_up_eq, 2up_shift_one_eq.
+          + rewrite 2shift_upRen_eq, 6shift_up_eq, liftSubst_can, 3singleSubstComm', 3up_shift_up_eq, 3 up_shift_one_eq.
+            do 4 f_equal. cbn.
+            now rewrite shift_up_eq, 3shift_one_eq. }
+      cbn in *.
+      14:{ (unshelve now eapply irrValidTm, Vn; eapply natValid); tea; now eapply lrefl. }
+      12:{ (unshelve now eapply irrValidTm, Vtl; eapply treeValid); tea; now eapply lrefl. }
+      7:{ (unshelve now eapply irrValidTm, Vtr; eapply treeValid); tea; now eapply lrefl. }
+      8: eapply VPn.
+      5: eapply VPtl.
+      2: eapply simpleArrValid, simpleArrValid, VPnode; eapply substS; tea.
+      1: eapply simpleArrValid, VPnode; eapply substS; tea.
+  Qed.
+
+
+End TreeElimRedValid.
+
+End Tree.
